docs/research/v8-full-view-zk-20260912/tools/run_r17_extracted_cm31.sh
@@ -46,6 +46,7 @@ case "$target" in
   AspisV8R17/GeneratedMulByR) ;;
   AspisV8R17/GeneratedQM31Products) ;;
   AspisV8R17/GeneratedQM31Linear) ;;
+  AspisV8R17/QM31WordFormulas|AspisV8R17/QM31WordResidues) ;;
   AspisV8R17/RawReducerNat|AspisV8R17/RawReducer) ;;
   *) exit 2 ;;
 esac
